

§ Lecture 25.0

Friday, 14 November 2025 20:11

Differentiability at a point:

Let $X \subseteq \mathbb{R}$. Let $x_0 \in X$ be a limit point of X .

Let $f: X \rightarrow \mathbb{R}$. If limit

$$\lim_{x \rightarrow x_0; x \in X - \{x_0\}} \frac{f(x) - f(x_0)}{x - x_0}$$

exists and is equal to L , then we say

that f is differentiable at x_0 on X with

derivative L .

$$f'(x_0) = L.$$

If limit doesn't exist

or if $x_0 \notin X$

or if x_0 is not a limit point of X

then f is not differentiable at x_0 on X .

[x_0 being a limit point is needed to define the limit]

Suppose $f(x) = x^2$ $x \in [1, 2] \cup \{3\}$

then function is not differentiable at $x_0 = 3$

on $[1, 2] \cup \{3\}$.

Ex 2 $f: \mathbb{R} \rightarrow \mathbb{R}$

$$f(x) = |x| \quad x_0 = 0$$

$$\lim_{x \rightarrow 0; x \in \mathbb{R} - \{0\}} \frac{f(x) - f(0)}{x - 0} = \lim_{x \rightarrow 0; x \in \mathbb{R} - \{0\}} \frac{|x|}{x}$$

The right hand limit

$$\lim_{x \rightarrow 0; x \in (0, \infty)} \frac{|x|}{x} = 1$$

left hand limit

$$\lim_{x \rightarrow 0; x \in (-\infty, 0)} \frac{|x|}{x} = -1$$

Thus $\lim_{x \rightarrow 0; x \in \mathbb{R} - \{0\}} \frac{f(x) - f(0)}{x}$ doesn't exist.

And function is not differentiable at 0 on \mathbb{R} .

Suppose we restrict the domain of f to $[0, \infty)$

then

$$\lim_{x \rightarrow 0; x \in [0, \infty) - \{0\}} \frac{f(x) - f(0)}{x} = \lim_{x \rightarrow 0; x \in (0, \infty)} \frac{|x|}{x} = 1$$

This function $f|_{[0, \infty)}$ is differentiable at 0 on $[0, \infty)$ with

derivative 1.

Differentiability implies continuity:

Let $X \subseteq \mathbb{R}$ and let $x_0 \in X$ be a limit point of X .

Let $f: X \rightarrow \mathbb{R}$ be a function. If f is differentiable at

x_0 then f is also continuous at x_0 .

Proof: Given that

$$\lim_{x \rightarrow x_0; x \in X - \{x_0\}} \frac{f(x) - f(x_0)}{x - x_0} := L \quad (\text{Exists})$$

Since x_0 is a limit point of X .

$\Rightarrow \exists$ a sequence $(x_n)_{n \geq 1}$ with $x_n \in X - \{x_0\}$ that

converges to $x_0 \in X$.

$$\text{Consider } f(x_n) - f(x_0) = \frac{f(x_n) - f(x_0)}{x_n - x_0} \times (x_n - x_0)$$

$(x_n \neq x_0 \forall n \geq 1)$

$$\lim_{n \rightarrow \infty} (f(x_n) - f(x_0)) = \lim_{n \rightarrow \infty} \left(\frac{f(x_n) - f(x_0)}{x_n - x_0} \right) \lim_{n \rightarrow \infty} (x_n - x_0)$$

$$= 0$$

$$\Rightarrow \lim_{n \rightarrow \infty} f(x_n) = f(x_0)$$

$\Rightarrow f$ is continuous at x_0 .

Proposition: (Newton's approximation)

Let $X \subseteq \mathbb{R}$. Let $x_0 \in X$ be a limit point of X . Let $f: X \rightarrow \mathbb{R}$

be a function. and $L \in \mathbb{R}$. Then following statements are equivalent.

(a) $f'(x_0) = L$.

(b) $\forall \varepsilon > 0 \exists \delta > 0$ s.t.

$$|f(x) - (f(x_0) + L(x - x_0))| \leq \varepsilon |x - x_0|$$

whenever $x \in X$ and $|x - x_0| \leq \delta$.

Proof: (a) \Rightarrow (b)

Given $\lim_{x \rightarrow x_0; x \in X - \{x_0\}} \frac{f(x) - f(x_0)}{x - x_0} = L$

$\Rightarrow \forall \varepsilon > 0 \exists \delta > 0$ s.t.

$$\left| \frac{f(x) - f(x_0)}{x - x_0} - L \right| \leq \varepsilon \quad \text{whenever } x \in X - \{x_0\} \text{ and } |x - x_0| \leq \delta.$$

$$\Rightarrow |f(x) - (f(x_0) + L(x - x_0))| \leq \varepsilon |x - x_0|.$$

For $x = x_0$, the inequality is trivially satisfied. Thus (b) is true.

(b) \Rightarrow (a)

Since (b) is true, for a fixed $\varepsilon > 0$ let $\delta > 0$ be

such that $\forall x \in X$ with $|x - x_0| \leq \delta$, we have

$$|f(x) - (f(x_0) + L(x - x_0))| \leq \varepsilon |x - x_0|$$

This is true for all $x \in X$ with $|x - x_0| \leq \delta$. we may

remove x_0 , we still have

$$\left| f(x) - (f(x_0) + L(x - x_0)) \right| \leq \varepsilon \quad \text{whenever} \\ |x - x_0| \leq \delta \quad \text{for } x \in X - \{x_0\}$$

$$\Rightarrow \left| \frac{f(x) - f(x_0)}{x - x_0} - L \right| \leq \varepsilon \quad \text{whenever} \\ |x - x_0| \leq \delta \quad \text{for } x \in X - \{x_0\}$$

$$\Rightarrow \lim_{x \rightarrow x_0; x \in X - \{x_0\}} \frac{f(x) - f(x_0)}{x - x_0} = L.$$

$$\Rightarrow f(x) \approx f(x_0) + (x - x_0) f'(x_0) \\ (\text{As long as } (x - x_0) \text{ is small}).$$

§ Lecture 25.1

Friday, 14 November 2025 21:11

Differential Calculus:

Premise: $X \subseteq \mathbb{R}$. $x_0 \in X$ be a limit point of X .

$f: X \rightarrow \mathbb{R}$ and $g: X \rightarrow \mathbb{R}$ be two functions.

(a) If $f(x) = c \ \forall x \in X$ then $f'(x_0) = 0$.

(b) If $f(x) = x \ \forall x \in X$ then $f'(x_0) = 1$

(c) If f and g are differentiable at x_0 then

$(f \pm g)$ is also differentiable at x_0 .

(d) If f, g are differentiable at x_0 then fg is

also differentiable at x_0 and

$$(fg)'(x_0) = f'(x_0)g(x_0) + f(x_0)g'(x_0)$$

(e) If g is differentiable at x_0 and $g(x) \neq 0 \ \forall x \in X$

then $1/g$ is also differentiable and

$$\left(\frac{1}{g}\right)'(x_0) = -\frac{g'(x_0)}{(g(x_0))^2}.$$

Proof: (a) $f(x) = c \ \forall x \in X$

$$\lim_{x \rightarrow x_0; x \in X - \{x_0\}} \frac{f(x) - f(x_0)}{x - x_0} = \lim_{x \rightarrow x_0; x \in X - \{x_0\}} \frac{c - c}{x - x_0} = 0.$$

$$(d) \quad \frac{(fg)(x) - (fg)(x_0)}{x - x_0} = \frac{f(x)g(x) - f(x_0)g(x_0)}{x - x_0}$$

$$= \frac{(f(x) - f(x_0))g(x) + f(x_0)(g(x) - g(x_0))}{(x - x_0)}$$

$$\lim_{x \rightarrow x_0; x \in X - \{x_0\}} \frac{fg(x) - fg(x_0)}{x - x_0} = f'(x_0)g(x_0) + f(x_0)g'(x_0).$$

$$(e) \quad \frac{1}{g}(x) - \frac{1}{g}(x_0) = \frac{g(x_0) - g(x)}{g(x)g(x_0)}$$

$$\frac{f(x) - f(x_0)}{x - x_0} = \frac{f'(x_0)}{(g(x_0))^2}$$

$$\lim_{x \rightarrow x_0; x \in X - \{x_0\}} \frac{f(x) - f(x_0)}{x - x_0} = - \frac{f'(x_0)}{(g(x_0))^2}$$

Chain rule:

Let $X, Y \subseteq \mathbb{R}$. Let $x_0 \in X$ and $y_0 \in Y$ be limit points of

X and Y , respectively. Let $f: X \rightarrow Y$ be a function such

that $f(x_0) = y_0$ and f is differentiable at x_0 .

Suppose $g: Y \rightarrow \mathbb{R}$ be a differentiable function at y_0 .

Then $g \circ f: X \rightarrow \mathbb{R}$ is differentiable at x_0 and

$$(g \circ f)'(x_0) = g'(y_0) f'(x_0).$$

Proof: We want to prove that

$\forall \varepsilon > 0 \quad \exists \delta > 0$ s.t.

$$|(g \circ f)(x) - g \circ f(x_0) - AB(x - x_0)| \leq \varepsilon |x - x_0| \rightarrow (1)$$

whenever $|x - x_0| \leq \delta$.

$$\text{where } A = f'(x_0) \quad B = g'(y_0) \quad y_0 = f(x_0).$$

Fix some $\varepsilon > 0$.

$$\text{Define } \varepsilon_1 = \min \left\{ 1, \frac{\varepsilon}{|A| + |B| + 1} \right\} \rightarrow (2)$$

Given since f is differentiable at x_0 , we have

$$|f(x) - f(x_0) - A(x - x_0)| \leq \varepsilon_1 |x - x_0|$$

$$\text{whenever } |x - x_0| \leq \delta_1 \quad (\text{for some } \delta_1) \rightarrow (3)$$

Note that

$$|f(x) - y_0| \leq |f(x) - y_0 - A(x - x_0)| + |A(x - x_0)|$$

$$\leq (|A| + \varepsilon_1) |x - x_0|$$

$$\rightarrow (4)$$

$$\text{whenever } |x - x_0| \leq \delta_1$$

Since f is differentiable at y_0

$\exists \delta_2 > 0$ s.t.

$$|g(f(x)) - g(y_0) - B(f(x) - y_0)| \leq \varepsilon_1 |f(x) - y_0|$$

whenever $|f(x) - y_0| \leq \delta_2$. $\rightarrow \textcircled{5}$

Pick η s.t. $(|A| + \varepsilon_1) \eta \leq \delta_2$

$$\delta = \min \{ \delta_1, \eta \}$$

Then $|x - x_0| \leq \delta \Rightarrow |x - x_0| \leq \delta_1$

$$\text{and } |f(x) - y_0| \leq (|A| + \varepsilon_1) \eta \leq \delta_2$$

Then eqⁿ $\textcircled{5}$ is valid & eqⁿ $\textcircled{3}$.

We have

$$\begin{aligned} & |g \circ f(x) - g(y_0) - AB(x - x_0)| \\ &= |g \circ f(x) - g(y_0) - B(f(x) - y_0) + B(f(x) - y_0) - AB(x - x_0)| \\ &\leq \varepsilon_1 |f(x) - y_0| + |B| \varepsilon_1 |x - x_0| \\ &\leq \varepsilon_1 (|A| + \varepsilon_1) |x - x_0| + |B| \varepsilon_1 |x - x_0| \\ &= \varepsilon_1 (|A| + |B| + \varepsilon_1) |x - x_0| \\ &\leq \varepsilon_1 (|A| + |B| + 1) |x - x_0| \\ &\leq \varepsilon |x - x_0| \end{aligned}$$

whenever $|x - x_0| \leq \delta$.

Thus $(f \circ g)'(x_0) = AB = f'(x_0) g'(y_0)$.

